@@ -497,3 +497,5 @@ import Xv6.LinkInstallTrans
 import Xv6.LogLedger
 import Xv6.ProofBeginOp
 import Xv6.LinkBeginOp
+import Xv6.ProofSysSync
+import Xv6.LinkSysSync
